doc/coq/simple/Syntax.v
@@ -400,6 +400,13 @@ Arguments MVal {T}.
 
 Definition memory T := list (T * expr_value T).
 
+Definition update_m {T X} m (t : T) (x : X) := (t, x) :: m.
+
+Definition empty_mem {T} : list T := [].
+
+Notation "p '!->' v ';' mem" := (update_m mem p v)
+                              (at level 100, v at next level, right associativity).
+
 Inductive config T :=
   | Cf (e : tm) (C : dy_ctx T) (m : memory T) (t : T)
   | Rs (V : dy_value T) (m : memory T) (t : T)
@@ -1145,3 +1152,333 @@ Proof.
   try rewrite IHC1;
   try rewrite IHC2; eauto.
 Qed.
+
+Generalizable Variables T BT AT.
+
+Fixpoint inject_ctx_mem `{Eq T} (Cout : dy_ctx T) (mem : memory T) :=
+  match mem with
+  | [] => []
+  | (t, v) :: tl =>
+    (t, inject_v Cout v) :: inject_ctx_mem Cout tl
+  end.
+
+Fixpoint delete_ctx_mem `{Eq T} (Cout : dy_ctx T) (mem : memory T) :=
+  match mem with
+  | [] => []
+  | (t, v) :: tl =>
+    (t, delete_v eqb Cout v) :: delete_ctx_mem Cout tl
+  end.
+
+Lemma delete_ctx_mem_eq `{Eq T} :
+  forall (Cout : dy_ctx T) (mem : memory T),
+         delete_ctx_mem Cout (inject_ctx_mem Cout mem) = mem.
+Proof.
+  induction mem; simpl; eauto.
+  repeat des_goal; clarify; rw.
+  destruct e; simpl.
+  pose proof (@delete_inject_eq T eqb) as RR.
+  rewrite RR; eauto.
+  intros; rewrite eqb_eq; eauto.
+Qed.
+
+Inductive link BT AT :=
+  | BF (t : BT)
+  | AF (t : AT)
+.
+
+Arguments BF {BT AT}.
+Arguments AF {BT AT}.
+
+Definition link_eqb `{Eq BT} `{Eq AT} (t t' : link BT AT) :=
+  match t, t' with
+  | BF t, BF t' => eqb t t'
+  | AF t, AF t' => eqb t t'
+  | _, _ => false
+  end.
+
+Lemma link_eqb_eq `{Eq BT} `{Eq AT} :
+  forall (t t' : link BT AT), link_eqb t t' = true <-> t = t'.
+Proof.
+  intros.
+  destruct t; destruct t'; simpl; split; intros EQ; 
+  try rewrite eqb_eq in *;
+  try inversion EQ;
+  subst; eauto.
+Qed.
+
+#[export] Instance link_eq `{Eq BT} `{Eq AT} : Eq (link BT AT) :=
+  {
+    eqb := link_eqb;
+    eqb_eq := link_eqb_eq;
+  }.
+
+Fixpoint filter_ctx_bf {BT AT} (C : dy_ctx (link BT AT)) :=
+  match C with
+  | [||] => [||]
+  | dy_binde x t C' =>
+    match t with
+    | BF t => dy_binde x t (filter_ctx_bf C')
+    | AF t => filter_ctx_bf C'
+    end
+  | dy_bindm M C' C'' => dy_bindm M (filter_ctx_bf C') (filter_ctx_bf C'')
+  end.
+
+Fixpoint filter_ctx_af {BT AT} (C : dy_ctx (link BT AT)) :=
+  match C with
+  | [||] => [||]
+  | dy_binde x t C' =>
+    match t with
+    | AF t => dy_binde x t (filter_ctx_af C')
+    | BF t => filter_ctx_af C'
+    end
+  | dy_bindm M C' C'' => dy_bindm M (filter_ctx_af C') (filter_ctx_af C'')
+  end.
+
+Definition filter_v_bf {BT AT} (v : expr_value (link BT AT)) :=
+  match v with
+  | Closure x e C => Closure x e (filter_ctx_bf C)
+  end.
+
+Definition filter_v_af {BT AT} (v : expr_value (link BT AT)) :=
+  match v with
+  | Closure x e C => Closure x e (filter_ctx_af C)
+  end.
+
+Fixpoint filter_mem_bf {BT AT} (mem : memory (link BT AT)) :=
+  match mem with
+  | [] => []
+  | (AF _, _) :: tl => filter_mem_bf tl
+  | (BF t, v) :: tl => (t, filter_v_bf v) :: filter_mem_bf tl
+  end.
+
+Fixpoint filter_mem_af {BT AT} (mem : memory (link BT AT)) :=
+  match mem with
+  | [] => []
+  | (AF t, v) :: tl => (t, filter_v_af v) :: filter_mem_af tl
+  | (BF _, _) :: tl => filter_mem_af tl
+  end.
+
+Fixpoint lift_ctx_bf {BT AT} C : dy_ctx (link BT AT) :=
+  match C with
+  | [||] => [||]
+  | dy_binde x t C' => dy_binde x (BF t) (lift_ctx_bf C')
+  | dy_bindm M C' C'' => dy_bindm M (lift_ctx_bf C') (lift_ctx_bf C'')
+  end.
+
+Definition lift_v_bf {BT AT} v : expr_value (link BT AT) :=
+  match v with
+  | Closure x e C => Closure x e (lift_ctx_bf C)
+  end.
+
+Fixpoint lift_mem_bf {BT AT} m : memory (link BT AT) :=
+  match m with
+  | [] => []
+  | (t, v) :: tl => (BF t, lift_v_bf v) :: lift_mem_bf tl
+  end.
+
+Fixpoint lift_ctx_af {BT AT} C : dy_ctx (link BT AT) :=
+  match C with
+  | [||] => [||]
+  | dy_binde x t C' => dy_binde x (AF t) (lift_ctx_af C')
+  | dy_bindm M C' C'' => dy_bindm M (lift_ctx_af C') (lift_ctx_af C'')
+  end.
+
+Definition lift_v_af {BT AT} v : expr_value (link BT AT) :=
+  match v with
+  | Closure x e C => Closure x e (lift_ctx_af C)
+  end.
+
+Fixpoint lift_mem_af {BT AT} m : memory (link BT AT) :=
+  match m with
+  | [] => []
+  | (t, v) :: tl => (AF t, lift_v_af v) :: lift_mem_af tl
+  end.
+
+Lemma read_filter_bf `{Eq BT} `{Eq AT} :
+  forall (m : memory (link BT AT)) (t : BT) (v : expr_value BT),
+    Some v = read (filter_mem_bf m) t <->
+    exists v', v = filter_v_bf v' /\ Some v' = read m (BF t).
+Proof.
+  induction m; ii;
+  split; intros READ; ss;
+  repeat des_goal; repeat des_hyp; des;
+  try rewrite eqb_eq in *;
+  try rewrite eqb_neq in *;
+  try rewrite link_eqb_eq in *;
+  clarify; eauto;
+  try rewrite <- aread_in in *;
+  first [ rewrite IHm in READ; des; eauto 
+        | try right; rewrite IHm; exists v'; eauto
+        | ss; rewrite eqb_neq in *; contradict].
+Qed.
+
+Lemma aread_filter_bf `{Eq BT} `{Eq AT} :
+  forall (m : memory (link BT AT)) (t : BT) (v : expr_value BT),
+    In v (aread (filter_mem_bf m) t) <->
+    exists v', v = filter_v_bf v' /\ In v' (aread m (BF t)).
+Proof.
+  induction m; ii; rewrite aread_in in *;
+  split; intros READ; ss;
+  repeat des_goal; repeat des_hyp; des;
+  try rewrite eqb_eq in *; 
+  try rewrite link_eqb_eq in *;
+  clarify; eauto;
+  try rewrite <- aread_in in *;
+  first [ rewrite IHm in READ; des; eauto 
+        | try right; rewrite IHm; exists v'; eauto
+        | ss; rewrite eqb_neq in *; contradict].
+Qed.
+
+Lemma read_filter_af `{Eq BT} `{Eq AT} :
+  forall (m : memory (link BT AT)) (t : AT) (v : expr_value AT),
+    Some v = read (filter_mem_af m) t <->
+    exists v', v = filter_v_af v' /\ Some v' = read m (AF t).
+Proof.
+  induction m; ii;
+  split; intros READ; ss;
+  repeat des_goal; repeat des_hyp; des;
+  try rewrite eqb_eq in *;
+  try rewrite eqb_neq in *;
+  try rewrite link_eqb_eq in *;
+  clarify; eauto;
+  try rewrite <- aread_in in *;
+  first [ rewrite IHm in READ; des; eauto 
+        | try right; rewrite IHm; exists v'; eauto
+        | ss; rewrite eqb_neq in *; contradict].
+Qed.
+
+Lemma aread_filter_af `{Eq BT} `{Eq AT} :
+  forall (m : memory (link BT AT)) (t : AT) (v : expr_value AT),
+    In v (aread (filter_mem_af m) t) <->
+    exists v', v = filter_v_af v' /\ In v' (aread m (AF t)).
+Proof.
+  induction m; ii; rewrite aread_in in *;
+  split; intros READ; ss;
+  repeat des_goal; repeat des_hyp; des;
+  try rewrite eqb_eq in *; 
+  try rewrite link_eqb_eq in *;
+  clarify; eauto;
+  try rewrite <- aread_in in *;
+  first [ rewrite IHm in READ; des; eauto 
+        | try right; rewrite IHm; exists v'; eauto
+        | ss; rewrite eqb_neq in *; contradict].
+Qed.
+
+Lemma read_delete `{Eq T} :
+  forall (m : memory T) (Cout : dy_ctx T) t v,
+    Some v = read (delete_ctx_mem Cout m) t <->
+    exists v', v = delete_v eqb Cout v' /\ Some v' = read m t.
+Proof.
+  induction m; intros; ss; split; intros READ;
+  des; try contradict; repeat des_hyp; des; ss; 
+  try rewrite eqb_eq in *; clarify;
+  try rewrite t_refl; ss; eauto;
+  first [ rewrite IHm in READ; des; eauto
+        | try right; rewrite IHm; exists v'; eauto].
+Qed.
+
+Lemma aread_delete `{Eq T} :
+  forall (m : memory T) (Cout : dy_ctx T) t v,
+    In v (aread (delete_ctx_mem Cout m) t) <->
+    exists v', v = delete_v eqb Cout v' /\ In v' (aread m t).
+Proof.
+  induction m; intros; ss; split; intros READ;
+  des; try contradict; repeat des_hyp; des; ss; 
+  try rewrite eqb_eq in *; clarify;
+  try rewrite t_refl; ss; eauto;
+  first [ rewrite IHm in READ; des; eauto
+        | try right; rewrite IHm; exists v'; eauto].
+Qed.
+
+Definition link_mem `{Eq BT} `{Eq AT}
+  (bmem : memory BT) (Cout : dy_ctx BT)
+  (amem : memory AT) : (memory (link BT AT)) :=
+  (inject_ctx_mem (lift_ctx_bf Cout) (lift_mem_af amem)) ++ 
+  (lift_mem_bf bmem).
+
+Lemma filter_lift_eq_af {BT AT} :
+  forall (C : dy_ctx AT),
+    filter_ctx_af (@lift_ctx_af BT AT C) = C.
+Proof.
+  induction C; simpl; repeat rw; eauto.
+Qed.
+
+Lemma filter_lift_eq_bf {BT AT} :
+  forall (C : dy_ctx BT),
+    filter_ctx_bf (@lift_ctx_bf BT AT C) = C.
+Proof.
+  induction C; simpl; repeat rw; eauto.
+Qed.
+
+Lemma filter_delete_eq `{Eq BT} `{Eq AT} (Cout : dy_ctx BT):
+  forall bmem amem,
+  filter_mem_af
+    (delete_ctx_mem (lift_ctx_bf Cout)
+    (link_mem bmem Cout amem)) = amem.
+Proof.
+  induction amem; unfold link_mem;
+  ss; repeat des_goal; unfold delete_v;
+  ss; repeat des_goal.
+  - induction bmem; simpl; eauto.
+    des_goal; clarify.
+  - destruct e; ss; clarify.
+    rewrite delete_inject_eq.
+    rewrite filter_lift_eq_af.
+    unfold link_mem in *. rewrite IHamem. eauto.
+    intros. rewrite link_eqb_eq. eauto.
+Qed.
+
+Lemma link_update_m_eq `{Eq BT} `{Eq AT} (Cout : dy_ctx BT):
+  forall bmem amem (t : AT) v,
+  (AF t !-> inject_v (lift_ctx_bf Cout) (lift_v_af v);
+    (link_mem bmem Cout amem)) =
+    link_mem bmem Cout (t !-> v; amem).
+Proof.
+  intros. ss.
+Qed.
+
+Lemma lift_addr_x {BT AT} :
+  forall (C : @dy_ctx AT) x,
+    addr_x (lift_ctx_af C : @dy_ctx (@link BT AT)) x =
+      match addr_x C x with
+      | Some addr => Some (AF addr)
+      | None => None
+      end.
+Proof.
+  induction C; simpl; eauto;
+  intros;
+  repeat des_goal; repeat des_hyp;
+  try rewrite eqb_ID_eq in *; clarify;
+  repeat rw; eauto.
+Qed.
+
+Lemma lift_ctx_M {BT AT} :
+  forall (C : dy_ctx AT) M,
+    ctx_M (lift_ctx_af C : dy_ctx (link BT AT)) M =
+      match ctx_M C M with
+      | Some CM => Some (lift_ctx_af CM)
+      | None => None
+      end.
+Proof.
+  induction C; simpl; eauto;
+  intros;
+  repeat des_goal; repeat des_hyp;
+  try rewrite eqb_ID_eq in *; clarify;
+  repeat rw; eauto.
+Qed.
+
+Definition inject_cf `{Eq BT} `{Eq AT} (Cout : dy_ctx BT) (bmem : memory BT) (cf : config AT) :=
+  match cf with
+  | Cf e C m t =>
+    Cf e ((lift_ctx_af C)[|(lift_ctx_bf Cout)|])
+      (link_mem bmem Cout m) (AF t)
+  | Rs V m t =>
+    let m := link_mem bmem Cout m in
+    let t := AF t in
+    match V with
+    | EVal (Closure x e C) =>
+      Rs (EVal (Closure x e ((lift_ctx_af C)[|(lift_ctx_bf Cout)|]))) m t
+    | MVal C =>
+      Rs (MVal ((lift_ctx_af C)[|(lift_ctx_bf Cout)|])) m t
+    end
+  end.
